Finished pqremove() and pqdownheap().

code/Yazi.Tree.Types.fsti
@@ -2,6 +2,8 @@ module Yazi.Tree.Types
 
 module B = LowStar.Buffer
 module CB = LowStar.ConstBuffer
+module Seq = FStar.Seq
+module ST = FStar.HyperStack.ST
 module U16 = FStar.UInt16
 module U32 = FStar.UInt32
 module U8 = FStar.UInt8
@@ -42,6 +44,38 @@ type tree_heap_t = B.lbuffer U32.t (2 * U32.v l_codes + 1)
 
 type heap_len_t = l: U32.t{0 < U32.v l /\ U32.v l < U32.v heap_size}
 
+noextract
+type tree_len_t = tl: Ghost.erased nat{tl <= U32.v heap_size}
+
+type tree_depth_t = B.lbuffer U8.t (2 * U32.v l_codes + 1)
+
+// noextract
+// type cmp_spec_t =
+//     tree_len: nat 
+//   -> tree: Seq.seq ct_data{Seq.length tree == tree_len}
+//   -> depth: Seq.seq U8.t{Seq.length depth == 2 * U32.v l_codes + 1}
+//   -> i: U32.t
+//   -> j: U32.t
+//   -> Pure bool
+//   (requires (
+//     let open U32 in
+//     v i < tree_len /\ v i < Seq.length depth /\
+//     v j < tree_len /\ v j < Seq.length depth))
+//   (ensures fun _ -> True)
+
+// type cmp_impl (spec: cmp_spec_t) =
+//     tree_len: tree_len_t
+//   -> tree: B.lbuffer ct_data (Ghost.reveal tree_len)
+//   -> depth: tree_depth_t
+//   -> n: U32.t
+//   -> m: U32.t
+//   -> ST.Stack bool
+//   (requires fun h ->
+//     U32.v n < tree_len /\ U32.v m < tree_len /\ B.live h tree /\ B.live h depth)
+//   (ensures fun h0 res h1 ->
+//     B.modifies B.loc_none h0 h1 /\
+//     (res == true <==> spec tree_len (B.as_seq h1 tree) (B.as_seq h1 depth) n m))
+
 type heap_index_t (hl: heap_len_t) = i: U32.t{
   0 < U32.v i /\ U32.v i <= U32.v hl
 }
@@ -50,10 +84,22 @@ type heap_internal_index_t (hl: heap_len_t) = i: U32.t{
   0 < U32.v i /\ U32.v i <= U32.v hl / 2
 }
 
-noextract
-type tree_len_t = tl: Ghost.erased nat{tl <= U32.v heap_size}
+noeq type sort_ctx_t = {
+  // cmp_spec: Ghost.erased cmp_spec_t;
+  // cmp: cmp_impl cmp_spec;
+  
+  heap: tree_heap_t;
+  tree_len: tree_len_t;
+  tree: B.buffer ct_data;
 
-type tree_depth_t = B.lbuffer U8.t (2 * U32.v l_codes + 1)
+  depth: tree_depth_t;
+}
+
+type sort_ctx = ctx: CB.const_buffer sort_ctx_t{
+  ~ (B.g_is_null (CB.as_mbuf ctx)) /\ CB.length ctx == 1
+}
+
+type sort_state = B.lbuffer U32.t 2
 
 type lit_bufsize_t = s: U32.t {
   let open U32 in
@@ -74,9 +120,9 @@ type tree_context = {
   d_desc: tree_desc;
   bl_desc: tree_desc;
 
-  bl_count: bl_count_t;
-  heap: tree_heap_t;
-  depth: tree_depth_t;
+  // bl_count: bl_count_t;
+  // heap: tree_heap_t;
+  // depth: tree_depth_t;
 
   l_buf: B.buffer U8.t;
   d_buf: B.buffer U8.t;
