specs/Spec.Heap.fst
@@ -2,8 +2,10 @@ module Spec.Heap
 
 module B = LowStar.Buffer
 module C = Yazi.Deflate.Constants
+module CB = LowStar.ConstBuffer
 module HS = FStar.HyperStack
 module Math = FStar.Math.Lemmas
+module Seq = FStar.Seq
 module U16 = FStar.UInt16
 module U32 = FStar.UInt32
 module U8 = FStar.UInt8
@@ -14,16 +16,16 @@ open Lib.Seq
 open Yazi.Deflate.Constants
 open Yazi.Tree.Types
 
-type cmp_spec =
-    tl: nat 
-  -> tree: Seq.seq ct_data{Seq.length tree == tl}
-  -> depth: Seq.seq U8.t{Seq.length depth == 2 * U32.v C.l_codes + 1}
-  -> i: U32.t{U32.v i < tl /\ U32.v i < length depth}
-  -> j: U32.t{U32.v j < tl /\ U32.v j < length depth}
-  -> Tot bool
+private let heap_elem (tree_len: tree_len_t) (a: U32.t) =
+  U32.v a < tree_len && U32.v a < 2 * U32.v l_codes + 1
 
-val build_cmp: cmp_spec
-let build_cmp tl tree depth i j =
+let node_smaller
+  (tree_len: nat{tree_len <= U32.v heap_size})
+  (tree: Seq.seq ct_data{Seq.length tree == tree_len})
+  (depth: Seq.seq U8.t{Seq.length depth == 2 * U32.v l_codes + 1})
+  (i: U32.t{heap_elem tree_len i})
+  (j: U32.t{heap_elem tree_len j}):
+  Tot bool =
   let open U32 in
   let fi = U16.v (tree.[v i]).freq_or_code in
   let fj = U16.v (tree.[v j]).freq_or_code in
@@ -31,51 +33,300 @@ let build_cmp tl tree depth i j =
   (fi = fj && U8.v depth.[v i] < U8.v depth.[v j]) ||
   (fi = fj && U8.v depth.[v i] = U8.v depth.[v j] && v i <= v j))
 
-let heap_elem (tl: tree_len_t) (depth: tree_depth_t) (a: U32.t) =
-  U32.v a < tl /\ U32.v a < B.length depth
+unfold let get_heap_len (h: HS.mem) (state: sort_state) = U32.v (B.get h state 0)
+unfold let get_heap_max (h: HS.mem) (state: sort_state) = U32.v (B.get h state 1)
+
+let context_live (h: HS.mem) (ctx: sort_ctx) (state: sort_state) =
+  CB.live h ctx /\ ~ (B.g_is_null (CB.as_mbuf ctx)) /\ B.live h state /\
+  (let ctx' = B.get h (CB.as_mbuf ctx) 0 in
+  let heap_len = get_heap_len h state in
+  let heap_max = get_heap_max h state in
+  let heap = B.as_seq h ctx'.heap in
+  let tree = B.as_seq h ctx'.tree in
+  let depth = B.as_seq h ctx'.depth in
+  B.live h ctx'.heap /\ B.live h ctx'.tree /\ B.live h ctx'.depth /\
+  ~ (B.g_is_null ctx'.heap) /\ ~ (B.g_is_null ctx'.tree) /\ ~ (B.g_is_null ctx'.depth) /\
+
+  (let ctx = CB.as_mbuf ctx in
+  B.disjoint ctx state /\ B.disjoint ctx ctx'.tree /\ B.disjoint ctx ctx'.heap /\
+  B.disjoint ctx ctx'.depth /\ B.disjoint state ctx'.tree /\
+  B.disjoint state ctx'.heap /\ B.disjoint state ctx'.depth /\
+  B.disjoint ctx'.tree ctx'.heap /\ B.disjoint ctx'.tree ctx'.depth /\
+  B.disjoint ctx'.heap ctx'.depth) /\
+
+  B.length ctx'.tree == Ghost.reveal ctx'.tree_len /\
+  heap_len < heap_max /\ heap_max <= U32.v heap_size /\
+  (forall i. {:pattern (heap.[i])}
+    (0 < i /\ i <= heap_len \/ heap_max <= i /\ i < U32.v heap_size) ==>
+    heap_elem ctx'.tree_len heap.[i]))
+
+let heap_seq (h: HS.mem) (ctx: sort_ctx) (state: sort_state): Ghost (Seq.seq U32.t)
+  (requires 0 < get_heap_len h state /\ get_heap_len h state < U32.v heap_size)
+  (ensures fun s -> Seq.length s == get_heap_len h state) =
+  let heap = B.as_seq h (B.get h (CB.as_mbuf ctx) 0).heap in
+  Seq.slice heap 1 (get_heap_len h state + 1)
+
+let sorted_seq (h: HS.mem) (ctx: sort_ctx) (state: sort_state): Ghost (Seq.seq U32.t)
+  (requires get_heap_max h state <= U32.v heap_size)
+  (ensures fun s -> Seq.length s == U32.v heap_size - get_heap_max h state) =
+  let heap = B.as_seq h (B.get h (CB.as_mbuf ctx) 0).heap in
+  Seq.slice heap (get_heap_max h state) (U32.v heap_size)
+
+let element_seq (h: HS.mem) (ctx: sort_ctx) (state: sort_state): Ghost (Seq.seq U32.t)
+  (requires
+    0 < get_heap_len h state /\ get_heap_len h state < U32.v heap_size /\
+    get_heap_max h state <= U32.v heap_size)
+  (ensures fun s ->
+    let heap_len = get_heap_len h state in
+    let heap_max = get_heap_max h state in
+    Seq.length s == heap_len + U32.v heap_size - heap_max) =
+  heap_seq h ctx state @| sorted_seq h ctx state
+
+unfold let modifies_heap_only (h0 h1: HS.mem) (ctx: sort_ctx) (state: sort_state) =
+  let c = B.get h0 (CB.as_mbuf ctx) 0 in
+  B.modifies (B.loc_buffer c.heap) h0 h1 /\
+  context_live h0 ctx state /\ context_live h1 ctx state
+
+let whole_heap_perm (h0 h1: HS.mem) (ctx: sort_ctx) (state: sort_state): Tot Type0 =
+  let c0 = B.get h0 (CB.as_mbuf ctx) 0 in
+  Seq.permutation U32.t (B.as_seq h0 c0.heap) (B.as_seq h1 c0.heap)
+
+let heap_seq_perm (h0 h1: HS.mem) (ctx: sort_ctx) (state: sort_state):
+  Pure Type0
+  (requires
+    0 < get_heap_len h0 state /\ get_heap_len h0 state < U32.v heap_size /\
+    0 < get_heap_len h1 state /\ get_heap_len h1 state < U32.v heap_size)
+  (ensures fun _ -> True) =
+  Seq.permutation U32.t (heap_seq h0 ctx state) (heap_seq h1 ctx state)
+
+let sorted_seq_perm (h0 h1: HS.mem) (ctx: sort_ctx) (state: sort_state): Pure Type0
+  (requires
+    get_heap_max h0 state <= U32.v heap_size /\
+    get_heap_max h1 state <= U32.v heap_size)
+  (ensures fun _ -> True) =
+  Seq.permutation U32.t (sorted_seq h0 ctx state) (sorted_seq h1 ctx state)
+
+private unfold let element_seq_perm_pre (h0 h1: HS.mem) (state: sort_state) =
+  0 < get_heap_len h0 state /\ get_heap_len h0 state < U32.v heap_size /\
+  0 < get_heap_len h1 state /\ get_heap_len h1 state < U32.v heap_size /\
+  get_heap_max h0 state <= U32.v heap_size /\
+  get_heap_max h1 state <= U32.v heap_size
+
+let element_seq_perm (h0 h1: HS.mem) (ctx: sort_ctx) (state: sort_state):
+  Pure Type0
+  (requires element_seq_perm_pre h0 h1 state)
+  (ensures fun _ -> True) =
+  Seq.permutation U32.t (element_seq h0 ctx state) (element_seq h1 ctx state)
+
+let non_heap_unmodified (h0 h1: HS.mem) (ctx: sort_ctx) (state: sort_state) =
+  let heap = (B.get h1 (CB.as_mbuf ctx) 0).heap in
+  let heap0 = B.as_seq h0 heap in
+  let heap1 = B.as_seq h1 heap in
+  let heap_len = get_heap_len h0 state in
+  heap0.[0] == heap1.[0] /\
+  (forall i. i > heap_len ==> heap0.[i] == heap1.[i])
+
+let lemma_heap_seq_upd_perm
+  (h0 h1: HS.mem) (ctx: sort_ctx) (state: sort_state) (root i: U32.t): Lemma
+  (requires
+    (let c0 = B.get h0 (CB.as_mbuf ctx) 0 in
+    let heap0 = B.as_seq h0 c0.heap in
+    let heap_len = get_heap_len h0 state in
+    modifies_heap_only h0 h1 ctx state /\
+    whole_heap_perm h0 h1 ctx state /\
+    0 < heap_len /\
+    0 < U32.v root /\ U32.v root <= heap_len / 2 /\
+    i == heap0.[U32.v root] /\
+    non_heap_unmodified h0 h1 ctx state))
+  (ensures heap_seq_perm h0 h1 ctx state) =
+  let c0 = B.get h0 (CB.as_mbuf ctx) 0 in
+  let c1 = B.get h1 (CB.as_mbuf ctx) 0 in
+  let heap0 = B.as_seq h0 c0.heap in
+  let heap1 = B.as_seq h1 c1.heap in
+  let heap_len = get_heap_len h0 state in
+  let heap_size = U32.v heap_size in
+  assert(equal
+    (Seq.slice heap0 (heap_len + 1) heap_size)
+    (Seq.slice heap1 (heap_len + 1) heap_size));
+  permutation_split heap0 heap1 1 (heap_len + 1)
+
+let lemma_sorted_seq_unmodified_perm
+  (h0 h1: HS.mem) (ctx: sort_ctx) (state: sort_state): Lemma
+  (requires
+    modifies_heap_only h0 h1 ctx state /\
+    non_heap_unmodified h0 h1 ctx state)
+  (ensures sorted_seq_perm h0 h1 ctx state) =
+  assert(equal (sorted_seq h0 ctx state) (sorted_seq h1 ctx state))
+
+let lemma_element_seq_perm_append
+  (h0 h1: HS.mem) (ctx: sort_ctx) (state: sort_state): Lemma
+  (requires
+    modifies_heap_only h0 h1 ctx state /\
+    0 < get_heap_len h1 state /\
+    heap_seq_perm h0 h1 ctx state /\
+    sorted_seq_perm h0 h1 ctx state)
+  (ensures element_seq_perm h0 h1 ctx state) =
+  lemma_append_count (heap_seq h0 ctx state) (sorted_seq h0 ctx state);
+  lemma_append_count (heap_seq h1 ctx state) (sorted_seq h1 ctx state)
+
+private let rec heap_sorted'
+  (tree_len: nat{tree_len <= U32.v heap_size})
+  (tree: Seq.seq ct_data{Seq.length tree == tree_len})
+  (depth: Seq.seq U8.t{Seq.length depth == 2 * U32.v l_codes + 1})
+  (i: nat{i <= U32.v heap_size})
+  (heap: Seq.seq U32.t{
+    Seq.length heap == U32.v heap_size /\
+    (forall j. j >= i ==> heap_elem tree_len heap.[j])
+  }):
+  Tot bool
+  (decreases U32.v heap_size - i) =
+  if U32.v heap_size - i <= 1 then
+    true
+  else
+    if node_smaller tree_len tree depth heap.[i + 1] heap.[i] then
+      heap_sorted' tree_len tree depth (i + 1) heap
+    else
+      false
+
+let rec lemma_heap_sorted'
+  (tree_len: nat{tree_len <= U32.v heap_size})
+  (tree: Seq.seq ct_data{Seq.length tree == tree_len})
+  (depth: Seq.seq U8.t{Seq.length depth == 2 * U32.v l_codes + 1})
+  (i: nat{i <= U32.v heap_size})
+  (heap0: Seq.seq U32.t{
+    Seq.length heap0 == U32.v heap_size /\
+    (forall j. j >= i ==> heap_elem tree_len heap0.[j])
+  })
+  (heap1: Seq.seq U32.t{
+    Seq.length heap1 == U32.v heap_size /\
+    (forall j. j >= i ==> heap0.[j] == heap1.[j])
+  }):
+  Lemma
+  (requires heap_sorted' tree_len tree depth i heap0)
+  (ensures heap_sorted' tree_len tree depth i heap1)
+  (decreases U32.v heap_size - i) =
+  match U32.v heap_size - i with
+  | 0 -> ()
+  | _ -> lemma_heap_sorted' tree_len tree depth (i + 1) heap0 heap1
+
+unfold let heap_sorted (h: HS.mem) (ctx: sort_ctx) (state: sort_state):
+  Pure Type0
+  (requires context_live h ctx state)
+  (ensures fun _ -> True) =
+  let open U32 in
+  let ctx' = B.get h (CB.as_mbuf ctx) 0 in
+  let heap = B.as_seq h ctx'.heap in
+  let depth = B.as_seq h ctx'.depth in
+  let tree = B.as_seq h ctx'.tree in
+  let heap_len = get_heap_len h state in
+  let heap_max = get_heap_max h state in
+  
+  heap_max <= U32.v heap_size /\
+  (heap_len >= 1 /\ heap_max < U32.v heap_size ==> (forall j. 0 < j /\ j <= heap_len ==>
+    node_smaller ctx'.tree_len tree depth heap.[heap_max] heap.[j])) /\
+  heap_sorted' ctx'.tree_len tree depth heap_max heap
+
+#push-options "--z3rlimit 1024 --ifuel 1"
+private let rec lemma_heap_sorted_aux
+  (h: HS.mem) (ctx: sort_ctx) (state: sort_state) (i j: pos): Lemma
+  (requires (
+    context_live h ctx state /\ (
+    let heap_max = get_heap_max h state in
+    let ctx = B.get h (CB.as_mbuf ctx) 0 in
+    let tree = B.as_seq h ctx.tree in
+    let depth = B.as_seq h ctx.depth in
+    let heap = B.as_seq h ctx.heap in
+    heap_max <= i /\
+    i <= j /\ j < U32.v heap_size /\
+    heap_sorted' ctx.tree_len tree depth i heap)))
+  (ensures (
+    let ctx = B.get h (CB.as_mbuf ctx) 0 in
+    let tree = B.as_seq h ctx.tree in
+    let depth = B.as_seq h ctx.depth in
+    let heap = B.as_seq h ctx.heap in
+    heap_sorted' ctx.tree_len tree depth j heap))
+  (decreases j - i) =
+  match j - i with
+  | 0 | 1 -> ()
+  | _ ->
+    let heap_max = get_heap_max h state in
+    let ctx' = B.get h (CB.as_mbuf ctx) 0 in
+    let tree = B.as_seq h ctx'.tree in
+    let depth = B.as_seq h ctx'.depth in
+    let heap = B.as_seq h ctx'.heap in
+    lemma_heap_sorted_aux h ctx state (i + 1) j
+
+let rec lemma_heap_sorted
+  (h: HS.mem) (ctx: sort_ctx) (state: sort_state) (i j: pos): Lemma
+  (requires
+    context_live h ctx state /\
+    heap_sorted h ctx state /\
+    get_heap_max h state <= i /\ i <= j /\ j < U32.v heap_size)
+  (ensures (
+    let ctx = B.get h (CB.as_mbuf ctx) 0 in
+    let heap = B.as_seq h ctx.heap in
+    let depth = B.as_seq h ctx.depth in
+    let tree = B.as_seq h ctx.tree in
+    node_smaller ctx.tree_len tree depth heap.[j] heap.[i]
+  ))
+  (decreases j - i) =
+  let ctx' = B.get h (CB.as_mbuf ctx) 0 in
+  let heap = B.as_seq h ctx'.heap in
+  let depth = B.as_seq h ctx'.depth in
+  let tree = B.as_seq h ctx'.tree in
+  let heap_max = get_heap_max h state in
+  match j - i with
+  | 0 -> ()
+  | _ ->
+    lemma_heap_sorted_aux h ctx state heap_max i;
+    lemma_heap_sorted_aux h ctx state i j;
+    lemma_heap_sorted h ctx state (i + 1) j
+#pop-options
 
 let partial_well_formed
-  (cmp: cmp_spec) (h: HS.mem)
-  (heap: tree_heap_t) (hl: heap_len_t)
-  (tl: tree_len_t) (tree: B.lbuffer ct_data tl) (depth: tree_depth_t)
-  (i: heap_index_t hl) =
+  (h: HS.mem) (ctx: sort_ctx) (state: sort_state) (i: U32.t): Pure Type0
+  (requires context_live h ctx state)
+  (ensures fun _ -> True) =
   let open U32 in
-  let hl = v hl in
-  let heap_elem = heap_elem tl depth in
-  let heap = B.as_seq h heap in
-  let tree = B.as_seq h tree in
-  let depth = B.as_seq h depth in
-  let smaller = cmp tl tree depth in
+  let ctx = B.get h (CB.as_mbuf ctx) 0 in
+  let heap_len = get_heap_len h state in
+  let heap = B.as_seq h ctx.heap in
+  let tree = B.as_seq h ctx.tree in
+  let depth = B.as_seq h ctx.depth in
+  let smaller = node_smaller ctx.tree_len tree depth in
+
+  0 < v i /\ v i <= heap_len /\
+  (forall (k: nat). v i <= k /\ k <= heap_len / 2 ==> (
+    (heap.[k] `smaller` heap.[k * 2]) /\
+    (k * 2 + 1 <= heap_len ==> heap.[k] `smaller` heap.[k * 2 + 1]))) /\
+
   (forall a. a `smaller` a) /\
   (forall a b. a `smaller` b /\ b `smaller` a ==> a == b) /\
   (forall a b c. a `smaller` b /\ b `smaller` c ==> a `smaller` c) /\
-  (forall a b. a `smaller` b \/ b `smaller` a) /\
-  (forall (j: pos). j <= hl ==> v heap.[j] < tl) /\
-  (forall (k: nat). (v i <= k /\ k <= hl) ==> (
-    heap_elem heap.[k] /\
-    (k * 2 <= hl ==>
-      heap_elem heap.[k * 2] /\ heap.[k] `smaller` heap.[k * 2]) /\
-    (k * 2 + 1 <= hl ==>
-      heap_elem heap.[k * 2 + 1] /\ heap.[k] `smaller` heap.[k * 2 + 1])))
+  (forall a b. a `smaller` b \/ b `smaller` a)
 
-let well_formed
-  (cmp: cmp_spec) (h: HS.mem)
-  (heap: tree_heap_t) (hl: heap_len_t)
-  (tl: tree_len_t) (tree: B.lbuffer ct_data tl) (depth: tree_depth_t) =
-  partial_well_formed cmp h heap hl tl tree depth 1ul
+let well_formed (h: HS.mem) (ctx: sort_ctx) (state: sort_state) =
+  context_live h ctx state /\ partial_well_formed h ctx state 1ul
 
-unfold let permutation_partial (h1 h2: seq U32.t) (root hole: U32.t) =
+let permutation_partial (h1 h2: seq U32.t) (root hole: U32.t) =
   let root = U32.v root in let hole = U32.v hole in
+  (* h1 is the initial heap and the root of h1 is the element to be inserted to
+     the heap.*)
   length h1 == length h2 /\
   root <= hole /\ hole < length h1 /\
   (hole == root ==> Seq.permutation U32.t h1 h2 /\ h1 == h2) /\
   (hole <> root ==> 
+    (* Intermediate state. *)
     (h2.[hole] <> h1.[root] ==>
       count h1.[root] h2 + 1 == count h1.[root] h1 /\
       count h2.[hole] h2 == count h2.[hole] h1 + 1) /\
+
+    (* The initial status, the counts should be the same. *)
     (h2.[hole] == h1.[root] ==> count h1.[root] h2 == count h1.[root] h1) /\
+    
+    (* For other non-root elements, thier counts are unchanged. *)
     (forall (x: U32.t). {:pattern (count x h1) \/ (count x h2)}
-      (x <> h1.[root] /\ x <> h2.[hole]) ==> count x h1 == count x h2))
+      x <> h1.[root] /\ x <> h2.[hole] ==> count x h1 == count x h2))
 
 private let rec log2 (a: pos): Tot (n: nat{
   pow2 n <= a /\ a < pow2 (n + 1)
@@ -98,53 +349,146 @@ private let rec log2_pow2_gt (a: pos) (n: pos): Lemma
 private let rec parent (a: pos) (i: pos{i <= log2 a}): Tot (res: pos{res < a}) =
   if i > 1 then parent (a / 2) (i - 1) else a / 2
 
-private let rec parent_next (a: pos) (i: pos{1 < i /\ i <= log2 a}): Lemma
+private let rec lemma_parent_next (a: pos) (i: pos{1 < i /\ i <= log2 a}): Lemma
   (ensures parent a i == parent a (i - 1) / 2) =
   match i with
   | 2 -> ()
-  | _ -> parent_next (a / 2) (i - 1)
+  | _ -> lemma_parent_next (a / 2) (i - 1)
 
-#set-options "--z3refresh --z3rlimit 512 --fuel 1 --ifuel 0"
-private let rec partial_well_formed_max
-  (cmp: cmp_spec) (h: HS.mem)
-  (heap: tree_heap_t) (hl: heap_len_t)
-  (tl: tree_len_t) (tree: B.lbuffer ct_data tl) (depth: tree_depth_t)
-  (i: nat) (j: pos) : Lemma
+private let lemma_div2 (a b: nat): Lemma
+  (requires a / 2 == b)
+  (ensures b * 2 == a \/ b * 2 + 1 == a) = ()
+
+#set-options "--z3refresh --z3rlimit 1024 --fuel 1 --ifuel 0 --z3seed 11"
+private let rec lemma_partial_well_formed_max
+  (h: HS.mem) (ctx: sort_ctx) (state: sort_state)
+  (height: nat) (j: pos) : Lemma
   (requires
-    i < log2 j /\ j <= U32.v hl /\ pow2 i < j /\
-    partial_well_formed cmp h heap hl tl tree depth (U32.uint_to_t (pow2 i)))
-  (ensures
-    pow2 i <= parent j ((log2 j) - i) /\
-    parent j ((log2 j) - i) < pow2 (i + 1) /\
-    cmp tl (B.as_seq h tree) (B.as_seq h depth)
-      (B.as_seq h heap).[parent j ((log2 j) - i)] (B.as_seq h heap).[j])
-  (decreases U32.v hl - pow2 i) =
-  if j < pow2 (i + 2) then begin
-    log2_pow2_lt j i;
-    log2_pow2_gt j (i + 2)
+    context_live h ctx state /\
+    (let ctx' = B.get h (CB.as_mbuf ctx) 0 in
+    height < log2 j /\ j <= get_heap_len h state /\ pow2 height < j /\
+    partial_well_formed h ctx state (U32.uint_to_t (pow2 height))))
+  (ensures (
+    let ctx = B.get h (CB.as_mbuf ctx) 0 in
+    let heap = B.as_seq h ctx.heap in
+    let depth = B.as_seq h ctx.depth in
+    let tree = B.as_seq h ctx.tree in
+    let pj = parent j (log2 j - height) in
+    pow2 height <= pj /\ pj < pow2 (height + 1) /\
+    node_smaller ctx.tree_len tree depth heap.[pj] heap.[j]))
+  (decreases get_heap_len h state - pow2 height) =
+  if j < pow2 (height + 2) then begin
+    log2_pow2_lt j height;
+    log2_pow2_gt j (height + 2);
+    lemma_div2 j (parent j (log2 j - height))
   end else begin
-    partial_well_formed_max cmp h heap hl tl tree depth (i + 1) j;
-    parent_next j ((log2 j) - i)
+    lemma_partial_well_formed_max h ctx state (height + 1) j;
+    lemma_parent_next j (log2 j - height);
+    Math.subtraction_is_distributive (log2 j) height 1;
+    lemma_div2 (parent j (log2 j - (height + 1))) (parent j (log2 j - height))
   end
 
-private let heap_max'
-  (cmp: cmp_spec) (h: HS.mem)
-  (heap: tree_heap_t) (hl: heap_len_t)
-  (tl: tree_len_t) (tree: B.lbuffer ct_data tl) (depth: tree_depth_t)
-  (i: pos{1 < i /\ i <= U32.v hl}) : Lemma
-  (requires well_formed cmp h heap hl tl tree depth)
-  (ensures cmp tl (B.as_seq h tree) (B.as_seq h depth)
-    (B.as_seq h heap).[1] (B.as_seq h heap).[i]) =
-  partial_well_formed_max cmp h heap hl tl tree depth 0 i
+private let lemma_heap_max'
+  (h: HS.mem) (ctx: sort_ctx) (state: sort_state)
+  (i: pos{1 < i /\ i <= get_heap_len h state}) : Lemma
+  (requires well_formed h ctx state)
+  (ensures (
+    let ctx = B.get h (CB.as_mbuf ctx) 0 in
+    let heap = B.as_seq h ctx.heap in
+    let depth = B.as_seq h ctx.depth in
+    let tree = B.as_seq h ctx.tree in
+    node_smaller ctx.tree_len tree depth heap.[1] heap.[i])) =
+  lemma_partial_well_formed_max h ctx state 0 i
 
-let heap_max
-  (cmp: cmp_spec) (h: HS.mem)
-  (heap: tree_heap_t) (hl: heap_len_t)
-  (tl: tree_len_t) (tree: B.lbuffer ct_data tl) (depth: tree_depth_t): Lemma
-  (requires well_formed cmp h heap hl tl tree depth)
+let lemma_heap_max (h: HS.mem) (ctx: sort_ctx) (state: sort_state): Lemma
+  (requires well_formed h ctx state)
   (ensures forall i.
-    let tree = B.as_seq h tree in
-    let depth = B.as_seq h depth in
-    let heap = B.as_seq h heap in
-    1 < i /\ i < U32.v hl ==> cmp tl tree depth heap.[1] heap.[i]) =
-  Classical.forall_intro (Classical.move_requires (heap_max' cmp h heap hl tl tree depth))
+    let ctx = B.get h (CB.as_mbuf ctx) 0 in
+    let heap = B.as_seq h ctx.heap in
+    let depth = B.as_seq h ctx.depth in
+    let tree = B.as_seq h ctx.tree in
+    1 < i /\ i <= get_heap_len h state ==>
+       node_smaller ctx.tree_len tree depth heap.[1] heap.[i])
+  [SMTPat (well_formed h ctx state)] =
+  Classical.forall_intro (Classical.move_requires (lemma_heap_max' h ctx state))
+
+let lemma_non_heap_unmodified
+  (h0 h1: HS.mem) (ctx: sort_ctx) (state: sort_state):
+  Lemma 
+  (requires (
+    let c0 = B.get h0 (CB.as_mbuf ctx) 0 in
+    let heap0 = B.as_seq h0 c0.heap in
+    let heap1 = B.as_seq h1 c0.heap in
+    modifies_heap_only h0 h1 ctx state /\
+    (forall i. i >= get_heap_max h0 state ==> heap0.[i] == heap1.[i]) /\
+    heap_sorted h0 ctx state))
+  (ensures (
+    let c1 = B.get h1 (CB.as_mbuf ctx) 0 in
+    let heap = B.as_seq h1 c1.heap in
+    let tree = B.as_seq h1 c1.tree in
+    let depth = B.as_seq h1 c1.depth in
+    let heap_max = get_heap_max h1 state in
+    heap_sorted' c1.tree_len tree depth (heap_max) heap
+  )) =
+  let heap_max = get_heap_max h0 state in
+  match U32.v heap_size - heap_max with
+  | 0 -> ()
+  | _ ->
+    let c0 = B.get h0 (CB.as_mbuf ctx) 0 in
+    let c1 = B.get h1 (CB.as_mbuf ctx) 0 in
+    let tree = B.as_seq h0 c0.tree in
+    let depth = B.as_seq h0 c0.depth in
+    let heap0 = B.as_seq h0 c0.heap in
+    let heap1 = B.as_seq h1 c1.heap in
+    lemma_heap_sorted' c0.tree_len tree depth heap_max heap0 heap1
+
+let heap_moved (h0 h1: HS.mem) (ctx: sort_ctx) (state: sort_state) =
+  let c = B.get h0 (CB.as_mbuf ctx) 0 in
+  B.modifies (B.loc_buffer c.heap `B.loc_union` B.loc_buffer state) h0 h1 /\
+  context_live h0 ctx state /\ context_live h1 ctx state /\
+  well_formed h0 ctx state /\ well_formed h1 ctx state /\
+  get_heap_len h0 state - 1 == get_heap_len h1 state /\
+  get_heap_max h0 state - 1 == get_heap_max h1 state /\
+  heap_sorted h1 ctx state /\
+  element_seq_perm h0 h1 ctx state
+
+let lemma_element_seq_swap (h0 h1: HS.mem) (ctx: sort_ctx) (state: sort_state): Lemma
+  (requires (
+    let heap = (B.get h0 (CB.as_mbuf ctx) 0).heap in
+    let heap0 = B.as_seq h0 heap in
+    let heap1 = B.as_seq h1 heap in
+    B.modifies (B.loc_buffer heap `B.loc_union` B.loc_buffer state) h0 h1 /\
+    context_live h0 ctx state /\ context_live h1 ctx state /\
+    element_seq_perm_pre h0 h1 state /\
+    get_heap_len h0 state - 1 == get_heap_len h1 state /\
+    get_heap_max h0 state - 1 == get_heap_max h1 state /\
+    (forall i. i <> 1 /\ i <> get_heap_max h1 state ==> heap0.[i] == heap1.[i]) /\
+    heap1.[1] == heap0.[get_heap_len h0 state] /\ heap1.[get_heap_max h1 state] == heap0.[1]))
+  (ensures element_seq_perm h0 h1 ctx state) =
+  let heap = (B.get h0 (CB.as_mbuf ctx) 0).heap in
+  let heap0 = B.as_seq h0 heap in
+  let heap1 = B.as_seq h1 heap in
+  let hs0 = heap_seq h0 ctx state in
+  let hs1 = heap_seq h1 ctx state in
+  let ss0 = sorted_seq h0 ctx state in
+  let ss1 = sorted_seq h1 ctx state in
+  let es0 = element_seq h0 ctx state in
+  let es1 = element_seq h1 ctx state in
+  let heap_len = get_heap_len h0 state in
+  let heap_max = get_heap_max h0 state in
+  assert(forall i. {:pattern hs0.[i]} hs0.[i] == heap0.[i + 1]);
+  assert(forall i. {:pattern hs1.[i]} hs1.[i] == heap1.[i + 1]);
+  assert(forall i. {:pattern hs1.[i] \/ hs0.[i]} 0 < i ==> hs1.[i] == hs0.[i]);
+  assert(forall i. {:pattern ss0.[i]} ss0.[i] == heap0.[i + heap_max]);
+  assert(forall i. {:pattern ss1.[i]} ss1.[i] == heap1.[i + heap_max - 1]);
+  assert(forall i. i > 0 ==> ss0.[i - 1] == ss1.[i]);
+  assert(forall i. {:pattern es0.[i]}
+    (i < heap_len ==> es0.[i] == hs0.[i]) /\
+    (heap_len <= i ==> es0.[i] == ss0.[i - heap_len]));
+  assert(forall i. {:pattern es1.[i]}
+    (i < heap_len - 1 ==> es1.[i] == hs1.[i]) /\
+    (heap_len - 1 <= i ==> es1.[i] == ss1.[i - (heap_len - 1)]));
+  assert(forall i. {:pattern es0.[i] \/ es1.[i]}
+    i <> 0 /\ i <> heap_len - 1 ==> es0.[i] == es1.[i]);
+  swap_equal es0 es1 0 (heap_len - 1);
+  Seq.lemma_swap_permutes es0 0 (heap_len - 1)
