specs/Spec.Kraft.fst
@@ -1,0 +1,278 @@
+module Spec.Kraft
+
+module Math = FStar.Math.Lemmas
+
+open FStar.Seq
+open FStar.Mul
+open Lib.Seq
+open Lib.Rational
+
+let rec lemma_max_leaf_count t =
+  match t with
+  | Node l r ->
+    lemma_max_leaf_count l;
+    lemma_max_leaf_count r;
+    Math.pow2_le_compat (height t - 1) (height l);
+    Math.pow2_le_compat (height t - 1) (height r)
+  | _ -> ()
+
+let rec bit_length_upper_bound (t: tree) (h: nat): Lemma
+  (ensures bit_length t h <= pow2 h)
+  [SMTPat (bit_length t h)] =
+  match (height t, h) with
+  | (0, _) | (_, 0) -> ()
+  | _ ->
+    bit_length_upper_bound (left t) (h - 1);
+    bit_length_upper_bound (right t) (h - 1)
+
+let rec lemma_non_full_bit_length t h =
+  match (height t, h) with
+  | (0, _) | (_, 0) -> ()
+  | _ ->
+    let l = left t in let r = right t in let h' = h - 1 in
+    assert(leaf_count l < pow2 h' \/ leaf_count r < pow2 h');
+    if leaf_count l < pow2 h' then begin
+      lemma_non_full_bit_length l h';
+      assert(exists i. i < h' /\ bit_length l i > 0 /\ (i + 1) < h /\ bit_length t (i + 1) > 0)
+    end;
+    if leaf_count r < pow2 h' then begin
+      lemma_non_full_bit_length r h';
+      assert(exists i. i < h' /\ bit_length r i > 0 /\ (i + 1) < h /\ bit_length t (i + 1) > 0)
+    end
+
+#set-options "--z3refresh --z3rlimit 32 --fuel 1 --ifuel 0"
+let rec lemma_kraft_sorted sym len i j =
+  match length len with
+  | 2 -> ()
+  | _ ->
+    let len' = tail len in let sym' = tail sym in
+    cons_head_tail sym;
+    assert(forall k. {:pattern len.[k] \/ len'.[k - 1]} k > 0 ==> len.[k] == len'.[k - 1]);
+    if 0 < i then
+      lemma_kraft_sorted sym' len' (i - 1) (j - 1)
+    else if i < j then
+      lemma_kraft_sorted sym' len' 0 (j - 1)
+    else
+      ()
+#reset-options
+
+let kraft_code_rat (sym: sym_seq) (len: len_seq) (i: nat): Pure rat
+  (requires kraft_cond sym len /\ i < length len)
+  (ensures fun _ -> True) =
+  if i = 0 then
+    zero
+  else
+    sigma 0 (i - 1) (fun j -> (pow2 len.[i], pow2 len.[j]))
+
+let lemma_kraft_code_rat_distr (sym: sym_seq) (len: len_seq) (i: pos): Lemma
+  (requires kraft_cond sym len /\ i < length len)
+  (ensures
+    kraft_code_rat sym len i =$
+    of_int (pow2 len.[i]) *$ sigma 0 (i - 1) (fun j -> 1, pow2 len.[j])) =
+  sigma_mul_distributivity 
+    0 (i - 1) (of_int (pow2 len.[i]))
+    (fun j -> (pow2 len.[i], pow2 len.[j]))
+    (fun j -> (1, pow2 len.[j]))
+
+let lemma_kraft_term_gt_zero (l: pos): Lemma
+  (ensures zero <$ (1, pow2 l))
+  [SMTPat (1, pow2 l)] = ()
+
+#set-options "--z3refresh --z3rlimit 128 --fuel 0 --ifuel 0"
+let lemma_kraft_code_rat_upper_bound
+  (sym: sym_seq) (len: len_seq) (i: nat): Lemma
+  (requires kraft_cond sym len /\ i < length len)
+  (ensures kraft_code_rat sym len i <$ (of_int (pow2 len.[i]))) =
+  let f = fun j -> 1, pow2 len.[j] in
+  let c = of_int (pow2 len.[i]) in
+  if 0 < i then
+    calc (<$) {
+      kraft_code_rat sym len i;
+      =={}
+      sigma 0 (i - 1) (fun j -> (pow2 len.[i], pow2 len.[j]));
+      =${lemma_kraft_code_rat_distr sym len i}
+      c *$ sigma 0 (i - 1) (fun j -> 1, pow2 len.[j]);
+      =${sigma_extensionality 0 (i - 1)  (fun j -> 1, pow2 len.[j]) f}
+      c *$ sigma 0 (i - 1) f;
+      <${
+        calc (<$) {
+          sigma 0 (i - 1) f;
+          <${sigma_pos_lt 0 (i - 1) (length len - 1) f}
+          sigma 0 (length len - 1) f;
+          =${}
+          kraft_sum len;
+          <=${}
+          one;
+        }
+      }
+      c;
+    }
+
+#set-options "--z3refresh --z3rlimit 128 --fuel 1 --ifuel 0"
+let rec lemma_kraft_code_rat_nat
+  (sym: sym_seq) (len: len_seq) (i j: nat): Lemma
+  (requires kraft_cond sym len /\ i < j /\ j < length len)
+  (ensures
+    sigma i (j - 1) (fun k -> (pow2 len.[j], pow2 len.[k])) =$
+    of_int (do_kraft_code sym len i j))
+  (decreases j - i) =
+  calc (<=) {
+    len.[i];
+    <={lemma_kraft_sorted sym len i j}
+    len.[j];
+  };
+  match j - i with
+  | 1 ->
+    calc (=$) {
+      sigma i (j - 1) (fun k -> pow2 len.[j], pow2 len.[k]);
+      =={}
+      (pow2 len.[j], pow2 len.[i]);
+      =${pow2_subtraction len.[j] len.[i]}
+      (pow2 (len.[j] - len.[i]), 1);
+      =={}
+      of_int (do_kraft_code sym len i j);
+    }
+  | _ ->
+    let f (k: nat{i <= k /\ k <= j - 1}): Tot rat =
+      pow2 len.[j], pow2 len.[k]
+    in
+    lemma_kraft_code_rat_nat sym len (i + 1) j;
+    sigma_extensionality (i + 1) (j - 1) f (fun k -> (pow2 len.[j], pow2 len.[k]));
+    calc (=$) {
+      sigma i (j - 1) f;
+      =${}
+      (pow2 len.[j], pow2 len.[i]) +$ of_int (do_kraft_code sym len (i + 1) j);
+      =${pow2_subtraction len.[j] len.[i]}
+      (pow2 (len.[j] - len.[i]), 1) +$ of_int (do_kraft_code sym len (i + 1) j);
+      =={}
+      (pow2 (len.[j] - len.[i]) + do_kraft_code sym len (i + 1) j, 1);
+      =={}
+      of_int (do_kraft_code sym len i j);
+    }
+
+let lemma_kraft_code_upper_bound sym len i =
+  if i > 0 then begin
+    lemma_kraft_code_rat_nat sym len 0 i;
+    lemma_kraft_code_rat_upper_bound sym len i
+  end
+
+#push-options "--z3refresh --z3rlimit 512 --fuel 2"
+let lemma_sigma_expand_1 (sym: sym_seq) (len: len_seq) (i j: nat): Lemma
+  (requires kraft_cond sym len /\ i + 1 == j /\ j < length len)
+  (ensures
+    sigma i j (fun k -> pow2 len.[j], pow2 len.[k]) ==
+    (pow2 len.[j], pow2 len.[i]) +$ (pow2 len.[j], pow2 len.[j])) = ()
+#pop-options
+
+#push-options "--fuel 1"
+let rec lemma_kraft_series_rat_extend (sym: sym_seq) (len: len_seq) (i j: nat): Lemma
+  (requires kraft_cond sym len /\ i < j /\ j < length len)
+  (ensures
+    sigma i j (fun k -> pow2 len.[j], pow2 len.[k]) =$
+    sigma i (j - 1) (fun k -> pow2 len.[j], pow2 len.[k]) +$ one)
+  (decreases j - i) =
+  match j - i with
+  | 1 ->
+    calc (=$) {
+      sigma i j (fun k -> pow2 len.[j], pow2 len.[k]);
+      =={lemma_sigma_expand_1 sym len i j}
+      (pow2 len.[j], pow2 len.[i]) +$ (pow2 len.[j], pow2 len.[j]);
+      =${}
+      (pow2 len.[j], pow2 len.[i]) +$ one;
+      =={}
+      sigma i (j - 1) (fun k -> pow2 len.[j], pow2 len.[k]) +$ one;
+    }
+  | _ ->
+    let f (k: nat{i <= k /\ k <= j}): Tot rat = pow2 len.[j], pow2 len.[k] in
+    calc (=$) {
+      sigma i j f;
+      =={}
+      (pow2 len.[j], pow2 len.[i]) +$ sigma (i + 1) j f;
+      =${sigma_extensionality (i + 1) j f (fun k -> pow2 len.[j], pow2 len.[k])}
+      (pow2 len.[j], pow2 len.[i]) +$ sigma (i + 1) j (fun k -> pow2 len.[j], pow2 len.[k]);
+      =${lemma_kraft_series_rat_extend sym len (i + 1) j}
+      (pow2 len.[j], pow2 len.[i]) +$
+      sigma (i + 1) (j - 1) (fun k -> pow2 len.[j], pow2 len.[k]) +$ one;
+      =${}
+      ((pow2 len.[j], pow2 len.[i]) +$
+      sigma (i + 1) (j - 1) (fun k -> pow2 len.[j], pow2 len.[k])) +$ one;
+      =${
+        sigma_extensionality (i + 1) (j - 1) f (fun k -> pow2 len.[j], pow2 len.[k]);
+        sigma_extensionality i (j - 1) f (fun k -> pow2 len.[j], pow2 len.[k])
+      }
+      sigma i (j - 1) (fun k -> pow2 len.[j], pow2 len.[k]) +$ one;
+    }
+#pop-options
+
+let lemma_kraft_code_rat_next (sym: sym_seq) (len: len_seq) (i: pos): Lemma
+  (requires kraft_cond sym len /\ i < length len)
+  (ensures
+    len.[i] >= len.[i - 1] /\
+    kraft_code_rat sym len i =$
+    (kraft_code_rat sym len (i - 1) +$ one) *$ of_int (pow2 (len.[i] - len.[i - 1]))) =
+  lemma_kraft_sorted sym len (i - 1) i;
+  if i > 1 then begin
+    let f (j: nat{0 <= j /\ j <= i - 1}): Tot rat = pow2 len.[i - 1], pow2 len.[j] in
+    calc (=$) {
+      kraft_code_rat sym len i;
+      =={}
+      sigma 0 (i - 1) (fun j -> pow2 len.[i], pow2 len.[j]);
+      =${
+        Math.pow2_plus (len.[i] - len.[i - 1]) len.[i - 1];
+        sigma_mul_distributivity
+          0 (i - 1)
+          (of_int (pow2 (len.[i] - len.[i - 1])))
+          (fun j -> pow2 len.[i], pow2 len.[j])
+          (fun j -> pow2 len.[i - 1], pow2 len.[j])
+      }
+      of_int (pow2 (len.[i] - len.[i - 1])) *$
+      sigma 0 (i - 1) (fun j -> pow2 len.[i - 1], pow2 len.[j]);
+      =${lemma_kraft_series_rat_extend sym len 0 (i - 1)}
+      of_int (pow2 (len.[i] - len.[i - 1])) *$
+      (sigma 0 (i - 1 - 1) (fun j -> pow2 len.[i - 1], pow2 len.[j]) +$ one);
+      =${
+        sigma_extensionality 0 (i - 1 - 1) f (fun j -> pow2 len.[i - 1], pow2 len.[j]);
+        assert(kraft_code_rat sym len (i - 1) =$
+          sigma 0 (i - 1 - 1) (fun j -> pow2 len.[i - 1], pow2 len.[j]))
+      }
+      of_int (pow2 (len.[i] - len.[i - 1])) *$ (kraft_code_rat sym len (i - 1) +$ one);
+    }
+  end else
+    calc (=$) {
+      kraft_code_rat sym len i;
+      =={}
+      (pow2 len.[1], pow2 len.[0]);
+      =${pow2_subtraction len.[1] len.[0]}
+      (pow2 (len.[1] - len.[0]), 1);
+      =${}
+      one *$ (pow2 (len.[1] - len.[0]), 1);
+      =${}
+      one *$ of_int (pow2 (len.[1] - len.[0]));
+    }
+
+let lemma_kraft_code_next sym len i =
+  lemma_kraft_sorted sym len (i - 1) i;
+  if i > 1 then
+    let f (j: nat{0 <= j /\ j <= i - 1}): Tot rat = pow2 len.[i - 1], pow2 len.[j] in
+    calc (=$) {
+      of_int (do_kraft_code sym len 0 i);
+      =${lemma_kraft_code_rat_nat sym len 0 i}
+      sigma 0 (i - 1) (fun j -> (pow2 len.[i], pow2 len.[j]));
+      =={}
+      kraft_code_rat sym len i;
+      =${lemma_kraft_code_rat_next sym len i}
+      of_int (pow2 (len.[i] - len.[i - 1])) *$
+      (kraft_code_rat sym len (i - 1) +$ one);
+      =${
+        sigma_extensionality 0 (i - 1 - 1) f (fun j -> pow2 len.[i - 1], pow2 len.[j]);
+        assert(kraft_code_rat sym len (i - 1) =$
+          sigma 0 (i - 1 - 1) (fun j -> pow2 len.[i - 1], pow2 len.[j]))
+      }
+      of_int (pow2 (len.[i] - len.[i - 1])) *$
+      (sigma 0 (i - 1 - 1) (fun j -> pow2 len.[i - 1], pow2 len.[j]) +$ one);
+      =${lemma_kraft_code_rat_nat sym len 0 (i - 1)}
+      of_int (pow2 (len.[i] - len.[i - 1])) *$
+      (of_int (do_kraft_code sym len 0 (i - 1) + 1));
+      =={}
+      of_int ((pow2 (len.[i] - len.[i - 1])) * (do_kraft_code sym len 0 (i - 1) + 1));
+    }
