specs/Spec.Kraft.fsti
@@ -1,0 +1,162 @@
+module Spec.Kraft
+
+module UInt = FStar.UInt
+module Math = FStar.Math.Lemmas
+
+open FStar.Mul
+open FStar.Seq
+open Lib.Seq
+open Lib.Rational
+
+type tree = 
+  | Node: left: tree -> right: tree -> tree
+  | Leaf: symbol: nat -> tree
+
+type non_leaf = t: tree{Leaf? t == false}
+
+unfold let left (t: non_leaf) =
+  match t with
+  | Node l _ -> l
+
+unfold let right (t: non_leaf) =
+  match t with
+  | Node _ r -> r
+
+let rec height (t: tree): Tot nat =
+  match t with
+  | Node l r ->
+    let lh = height l in let rh = height r in
+    1 + (if lh > rh then lh else rh)
+  | _ -> 0
+
+let rec leaf_count (t: tree): Tot pos = 
+  match t with
+  | Node l r -> leaf_count l + leaf_count r
+  | _ -> 1
+
+let max_leaf_count (t: tree): Tot pos = pow2 (height t)
+
+let rec bit_length (t: tree) (h: nat): Tot nat =
+  match t with
+  | Node l r ->
+    if h = 0 then 0 else bit_length l (h - 1) + bit_length r (h - 1)
+  | _ ->
+    if h = 0 then 1 else 0
+
+val lemma_max_leaf_count: (t: tree) -> Lemma
+  (ensures leaf_count t <= max_leaf_count t)
+
+val lemma_non_full_bit_length: (t: tree) -> (h: nat) -> Lemma
+  (requires leaf_count t < pow2 h)
+  (ensures exists i. i < h /\ bit_length t i > 0)
+
+let kraft_sum (len: seq pos): Tot rat =
+  if length len = 0 then
+    zero
+  else
+    sigma 0 (length len - 1) (fun j -> 1, pow2 len.[j])
+
+type sym_seq = sym: seq nat{
+  length sym >= 2 /\ no_dup sym
+}
+
+type len_seq = len: seq pos{
+  length len >= 2 /\ kraft_sum len <=$ one
+}
+
+let rec kraft_sorted
+  (sym: seq nat) (len: seq pos{length sym == length len}):
+  Tot bool (decreases length sym) =
+  if length sym <= 1 then
+    true
+  else
+    let (s1, s2) = (head sym, sym.[1]) in
+    let (l1, l2) = (head len, len.[1]) in
+    (l1 < l2 || l1 = l2 && s1 < s2) && kraft_sorted (tail sym) (tail len)
+
+let kraft_cond (sym: sym_seq) (len: len_seq) =
+  length sym == length len /\ kraft_sorted sym len
+
+val lemma_kraft_sorted: sym: seq nat -> len: seq pos -> i: nat -> j: nat -> Lemma
+  (requires length sym == length len /\ kraft_sorted sym len /\ i <= j /\ j < length len)
+  (ensures len.[i] <= len.[j])
+  (decreases length len)
+
+private let rec do_kraft_code (sym: sym_seq) (len: len_seq) (i j: nat): Pure nat
+  (requires kraft_cond sym len /\ i < j /\ j < length len)
+  (ensures fun _ -> True)
+  (decreases j - i) =
+  lemma_kraft_sorted sym len i j;
+  if i + 1 = j then
+    pow2 (len.[j] - len.[i])
+  else
+    pow2 (len.[j] - len.[i]) + do_kraft_code sym len (i + 1) j
+
+let kraft_code (sym: sym_seq) (len: len_seq) (i: nat): Pure nat
+  (requires kraft_cond sym len /\ i < length len)
+  (ensures fun _ -> True) =
+  if i = 0 then 0 else do_kraft_code sym len 0 i
+
+val lemma_kraft_code_upper_bound:
+    (sym: sym_seq)
+  -> (len: len_seq)
+  -> (i: nat)
+  -> Lemma
+  (requires kraft_cond sym len /\ i < length len)
+  (ensures kraft_code sym len i < pow2 len.[i])
+  [SMTPat (kraft_code sym len i)]
+
+val lemma_kraft_code_next: sym: sym_seq -> len: len_seq -> i: pos -> Lemma
+  (requires kraft_cond sym len /\ i < length len)
+  (ensures
+    len.[i] >= len.[i - 1] /\
+    kraft_code sym len i ==
+    (kraft_code sym len (i - 1) + 1) * pow2 (len.[i] - len.[i - 1]))
+
+#push-options "--fuel 0"
+let kraft_code_uint (sym: sym_seq) (len: len_seq) (i: nat{i < length len}):
+  Pure (UInt.uint_t len.[i])
+  (requires kraft_cond sym len)
+  (ensures fun c -> c == kraft_code sym len i) =
+  if i = 0 then
+    0
+  else begin
+    lemma_kraft_sorted sym len (i - 1) i;
+    lemma_kraft_code_upper_bound sym len i;
+    lemma_kraft_code_next sym len i;
+    let c = UInt.shift_left
+      #len.[i]
+      (kraft_code sym len (i - 1) + 1)
+      (len.[i] - len.[i - 1])
+    in
+    calc (==) {
+      kraft_code sym len i;
+      =={
+        Math.modulo_lemma (kraft_code sym len i) (pow2 len.[i])
+      }
+      (kraft_code sym len i) % pow2 len.[i];
+      =={lemma_kraft_code_next sym len i}
+      ((kraft_code sym len (i - 1) + 1) * pow2 (len.[i] - len.[i - 1])) % pow2 len.[i];
+      =={
+        UInt.shift_left_value_lemma
+          #len.[i]
+          (kraft_code sym len (i - 1) + 1)
+          (len.[i] - len.[i - 1])
+      }
+      c;
+    };
+    c
+  end
+#pop-options
+
+let prefix (#n #m: nat) (a: UInt.uint_t n) (b: UInt.uint_t m): bool =
+  if n > m then
+    false
+  else
+    let a' = UInt.to_vec a in
+    let b' = UInt.to_vec b in
+    slice a' 0 n = slice b' 0 n
+
+// val kraft_code_prefix: sym: sym_seq -> len: len_seq -> i: nat -> j: nat -> Lemma
+//   (requires kraft_cond sym len /\ i < j /\ j < length len)
+//   (ensures prefix a b == false)
